Add mlsexp datatype, conversions, factorization
Parts 1 and 2 of the TODO, and maybe all we need of part 3?
We've got the obvious iso between them, and the obvious factorization
theorems (duplicated somewhere else in more generality?), now the
question is what we can do with that.

botworld_preambleScript.sml
@@ -20,6 +20,47 @@ val _ = std_preludeLib.std_prelude();
       translator sees mlstring.
 *)
 
+val _ = Datatype `
+  mlsexp = sx_cons mlsexp mlsexp
+         | sx_sym mlstring
+         | sx_num num
+         | sx_str mlstring
+`
+
+val sexp_of_mls_def = Define `
+  sexp_of_mls (sx_cons s1 s2) = SX_CONS (sexp_of_mls s1) (sexp_of_mls s2) ∧
+  sexp_of_mls (sx_sym (strlit s)) = SX_SYM s ∧
+  sexp_of_mls (sx_num n) = SX_NUM n ∧
+  sexp_of_mls (sx_str (strlit s)) = SX_STR s
+`
+
+val mls_of_sexp_def = Define `
+  mls_of_sexp (SX_CONS s1 s2) = sx_cons (mls_of_sexp s1) (mls_of_sexp s2) ∧
+  mls_of_sexp (SX_SYM s) = sx_sym (strlit s) ∧
+  mls_of_sexp (SX_NUM n) = sx_num n ∧
+  mls_of_sexp (SX_STR s) = sx_str (strlit s)
+`
+
+val mls_sexp_inv = Q.prove(
+  `!s. mls_of_sexp (sexp_of_mls s) = s`,
+  rpt Induct >> rw[mls_of_sexp_def,sexp_of_mls_def]
+)
+
+val sexp_mls_inv = Q.prove(
+  `!s. sexp_of_mls (mls_of_sexp s) = s`,
+  rpt Induct >> rw[mls_of_sexp_def,sexp_of_mls_def]
+)
+
+val mlsexp_factors = Q.prove(
+  `!f. ?f'. f = f' o mls_of_sexp`,
+  rw[FUN_EQ_THM] >> qexists_tac `f o sexp_of_mls` >> rw[sexp_mls_inv]
+)
+
+val sexp_factors = Q.prove(
+  `!f. ?f'. f = f' o sexp_of_mls`,
+  rw[FUN_EQ_THM] >> qexists_tac `f o mls_of_sexp` >> rw[mls_sexp_inv]
+)
+
 val res = translate simpleSexpTheory.strip_sxcons_def;
 val res = translate simpleSexpParseTheory.print_space_separated_def;
 val res = translate simpleSexpParseTheory.escape_string_def;
